equational_theories/Duality.lean
@@ -1,0 +1,88 @@
+import equational_theories.Conjecture
+import equational_theories.FreeMagma
+
+universe u
+
+inductive DualMagma (α : Type u) [Magma α]
+  | DualWrap : α → DualMagma α
+
+def dualWrap {G : Type u} [Magma G] : (G → DualMagma G) := DualMagma.DualWrap
+
+def dualUnwrap {G : Type u} [Magma G] : (DualMagma G → G)
+  | DualMagma.DualWrap x => x
+
+instance {G : Type u} [Magma G] : Magma (DualMagma G) where
+  op x y := dualWrap $ (dualUnwrap y) ∘ (dualUnwrap x)
+
+-- TODO: Once we have an API for magma isomorphism, prove dualWrap and dualUnwrap are isomorphisms
+
+theorem DualMapIsAntihomomorphism (G : Type u) [Magma G] : ∀ x y : G, dualWrap (x ∘ y) = dualWrap y ∘ dualWrap x :=
+  fun _ _ ↦ refl _
+
+theorem DualMapCancellable (G : Type u) [Magma G] : ∀ x y : G, dualWrap x = dualWrap y → x = y :=
+  fun _ _ eq ↦ congrArg dualUnwrap eq
+
+theorem EvalReversedInDualMagma (G : Type u) [Magma G]
+  (expr : FreeMagma Nat) (sub : Nat → G) : dualWrap (evalInMagma sub expr) = evalInMagma (dualWrap ∘ sub) (dualizeTree expr) :=
+  match expr with
+  | FreeMagma.Leaf n => Eq.refl (dualWrap $ sub n)
+  | FreeMagma.Fork leftExpr rightExpr => by
+    let subd := dualWrap ∘ sub
+    have leftCase : dualWrap (evalInMagma sub leftExpr) = evalInMagma subd (dualizeTree leftExpr) := EvalReversedInDualMagma G leftExpr sub
+    have rightCase : dualWrap (evalInMagma sub rightExpr) = evalInMagma subd (dualizeTree rightExpr) := EvalReversedInDualMagma G rightExpr sub
+    have decompEval : evalInMagma sub (leftExpr ⋆ rightExpr) = (evalInMagma sub leftExpr) ∘ (evalInMagma sub rightExpr) := refl _
+    have decompDualEval : (evalInMagma subd (dualizeTree rightExpr) ∘ (evalInMagma subd (dualizeTree leftExpr))) = evalInMagma subd (dualizeTree (leftExpr ⋆ rightExpr)) := refl _
+    exact Eq.trans
+      (congrArg dualWrap decompEval) $ Eq.trans
+      (DualMapIsAntihomomorphism G _ _) $ Eq.trans
+      (congrArg (fun t ↦ t ∘ (dualWrap (evalInMagma sub leftExpr))) rightCase) $ Eq.trans
+      (congrArg (fun t ↦ (evalInMagma subd (dualizeTree rightExpr)) ∘ t) leftCase)
+      decompDualEval
+
+theorem EvalPreservedInDoubleDualMagma (G : Type u) [Magma G]
+  (expr : FreeMagma Nat) (sub : Nat → G) : dualWrap (dualWrap (evalInMagma sub expr)) = evalInMagma (dualWrap ∘ (dualWrap ∘ sub)) expr :=
+  Eq.trans
+    (congrArg dualWrap (EvalReversedInDualMagma G expr sub)) $ Eq.trans
+    (EvalReversedInDualMagma (DualMagma G) (dualizeTree expr) (dualWrap ∘ sub))
+    (congrArg (evalInMagma (dualWrap ∘ dualWrap ∘ sub)) (DualizeTreeIsInvolution expr))
+
+theorem DualizeLawFromMagma (G : Type u) [Magma G]
+  (law : EquationLaw) (pf : G ⊨ law) : DualMagma G ⊨ dualizeLaw law := by
+  intro subd
+  let sub := dualUnwrap ∘ subd
+  let subd' := dualWrap ∘ sub
+  have subEquiv : subd' = subd := funext (fun n ↦ congrArg dualWrap (refl _))
+  have eq : evalInMagma sub law.1 = evalInMagma sub law.2 := pf sub
+  have eqd' : evalInMagma subd' (dualizeTree law.1) = evalInMagma subd' (dualizeTree law.2) := Eq.trans
+    (Eq.symm $ EvalReversedInDualMagma G law.1 sub) $ Eq.trans
+    (congrArg dualWrap eq)
+    (EvalReversedInDualMagma G law.2 sub)
+  have eqd : evalInMagma subd (dualizeTree law.1) = evalInMagma subd (dualizeTree law.2) :=
+    Eq.rec (motive := fun f _ ↦ evalInMagma f (dualizeTree law.1) = evalInMagma f (dualizeTree law.2)) eqd' subEquiv
+  exact eqd
+
+theorem UndualizeLawFromDualMagma (G : Type u) [Magma G]
+  (law : EquationLaw) (dualPf : DualMagma G ⊨ dualizeLaw law) : G ⊨ law := by
+  intro sub
+  let subd := dualWrap ∘ sub
+  have dualLawSpecialized : evalInMagma subd (dualizeTree law.1) = evalInMagma subd (dualizeTree law.2) := dualPf subd
+  exact (DualMapCancellable G _ _ (Eq.trans
+    (EvalReversedInDualMagma G law.1 sub) $ Eq.trans
+    dualLawSpecialized
+    (Eq.symm $ EvalReversedInDualMagma G law.2 sub)))
+
+theorem DualizeLawFromDualMagma (G : Type u) [Magma G]
+  (law : EquationLaw) (dualPf : DualMagma G ⊨ law) : G ⊨ dualizeLaw law := by
+  have satDoubleDual : DualMagma G ⊨ dualizeLaw (dualizeLaw law) := Eq.ndrec dualPf (Eq.symm $ DualizeLawIsInvolution law)
+  exact (UndualizeLawFromDualMagma G (dualizeLaw law) satDoubleDual)
+
+theorem DualizeEquationLawImplication
+  (law1 law2 : EquationLaw) (imp : ∀ (G : Type u) [Magma G], G ⊨ law1 → G ⊨ law2)
+  : (∀ (H : Type u) [Magma H], H ⊨ dualizeLaw law1 → H ⊨ dualizeLaw law2) := by
+  intros G _ satDualLaw1
+  have dualSatLaw1 : DualMagma G ⊨ law1 := Eq.ndrec
+    (motive := fun l ↦ DualMagma G ⊨ l)
+    (DualizeLawFromMagma G (dualizeLaw law1) $ satDualLaw1)
+    (DualizeLawIsInvolution law1)
+  have dualSatLaw2 : DualMagma G ⊨ law2 := imp (DualMagma G) dualSatLaw1
+  exact (DualizeLawFromDualMagma G law2 dualSatLaw2)
